Diff/Robust2relSSCHPreservation.v
@@ -1,0 +1,153 @@
+From mathcomp Require Import all_ssreflect.
+
+Set Implicit Arguments.
+Unset Printing Implicit Defensive.
+
+Require Import ClassicalExtras.
+Require Import MyNotation.
+Require Import Setoid.
+Require Import FunctionalExtensionality.
+
+Require Import Galois.
+Require Import LanguageModel.
+Require Import TraceModel.
+Require Import Properties.
+Require Import ChainModel.
+
+Hypothesis prop_extensionality : forall A B : Prop, (A <-> B) -> A = B.
+
+Section Robust2relSSCHPreservation.
+
+  Variable Source Target: Language.
+  Variable compilation_chain : CompilationChain Source Target.
+
+  (*CA: we don't need a particular structure of traces to define preservation
+        e.g. traces = values or our defn of traces both make sense
+   *)
+  Variable trace__S trace__T : Set.
+
+  Local Definition prop__S := prop trace__S.
+  Local Definition prop__T := prop trace__T.
+
+  Variable Source_Semantics : Semantics Source trace__S.
+  Variable Target_Semantics : Semantics Target trace__T.
+
+  Local Definition sem__S := sem Source_Semantics.
+  Local Definition sem__T := sem Target_Semantics.
+  Local Definition beh__S := beh Source_Semantics.
+  Local Definition beh__T := beh Target_Semantics. 
+  Local Definition par__S := par Source.
+  Local Definition par__T := par Target.
+  Local Definition ctx__S := ctx Source.
+  Local Definition ctx__T := ctx Target. 
+  Local Definition rsat__S := rhsat2 Source_Semantics.
+  Local Definition rsat__T := rhsat2 Target_Semantics.
+  
+  Local Definition cmp := compile_par Source Target compilation_chain.
+
+  Local Notation "P ↓" := (cmp P) (at level 50).
+ (* CA: don't understand why this does not work 
+
+   Local Notation " C [ P ] " := (plug _  P C) (at level 50).
+  *)
+  Local Definition plug__S:= plug Source.
+  Local Definition plug__T := plug Target.
+
+  (* still mappings on trace properties *)
+  Variable σ__π : (trace__T -> Prop) -> (trace__S -> Prop).
+  Variable τ__π : (trace__S -> Prop) -> (trace__T -> Prop).
+
+  Definition σ : (prop__T * prop__T -> Prop) -> (prop__S * prop__S -> Prop) :=
+    fun T =>
+      fun Π => exists π__T π__T', fst Π = σ__π π__T /\
+                        snd Π = σ__π π__T /\
+                        T (π__T, π__T').
+
+  Definition τ : (prop__S * prop__S -> Prop) -> (prop__T * prop__T -> Prop) :=
+    fun S =>
+      fun Π => exists π__S π__S', fst Π = τ__π π__S /\
+                        snd Π = τ__π π__S /\
+                        S (π__S, π__S').
+  
+  Definition sCl_σ :  ((trace__T -> Prop) * (trace__T -> Prop) -> Prop) ->
+                      ((trace__S -> Prop) * (trace__S -> Prop) -> Prop) :=
+   sCl2  ∘ σ.
+  
+  Definition sCl_τ : ((trace__S -> Prop) * (trace__S -> Prop) -> Prop) ->
+                     ((trace__T -> Prop) * (trace__T -> Prop) -> Prop) :=
+   sCl2  ∘ τ.
+
+  Definition sCl_σR2rhP (P1 P2 : par__S) (T : prop__T * prop__T -> Prop) :=
+    rsat__S P1 P2 (sCl_σ T) -> rsat__T (P1 ↓) (P2 ↓) T.   
+
+  (* Lemma contra_σR2rhP (P1 P2 : par__S) (T : prop__T * prop__T -> Prop) : *)
+  (*   (σR2rhP P1 P2 T) <-> ((exists C__T, ~ T (beh__T (plug__T (P1 ↓) C__T), *)
+  (*                                     beh__T (plug__T (P2 ↓) C__T))) -> *)
+  (*                       (exists C__S, ~ (σ T) (beh__S (plug__S P1 C__S), *)
+  (*                                        beh__S (plug__S P2 C__S)))). *)
+  (* Proof. *)
+  (*   rewrite /sClσR2rhP. by rewrite [_ -> _] contra !neg_rhsat2. *)
+  (* Qed. *)
+
+  (* Lemma contra_σR2rHP : *)
+  (*   σR2rHP <-> (forall P1 P2 T, (exists C__T, ~ T (beh__T (plug__T (P1 ↓) C__T), *)
+  (*                                     beh__T (plug__T (P2 ↓) C__T))) -> *)
+  (*                         (exists C__S, ~ (σ T) (beh__S (plug__S P1 C__S), *)
+  (*                                        beh__S (plug__S P2 C__S)))). *)
+  (* Proof. *)
+  (*   rewrite /σR2rHP. *)
+  (*   split => H P1 P2 T; by move/contra_σR2rhP: (H P1 P2 T). *)
+  (* Qed. *)
+
+  Definition sCl_τR2rhP (P1 P2 : par__S) (S : prop__S * prop__S -> Prop) :=
+    rsat__S P1 P2 S -> rsat__T (P1 ↓) (P2 ↓) (sCl_τ S).
+  
+
+  (* Lemma contra_τR2rhP (P1 P2 : par__S) (S : prop__S * prop__S -> Prop) : *)
+  (*   (τR2rhP P1 P2 S) <-> ((exists C__T,  ~ (τ S) (beh__T (plug__T (P1 ↓) C__T), *)
+  (*                                         beh__T (plug__T (P2 ↓) C__T ))) -> *)
+  (*                     (exists C__S, ~ S (beh__S (plug__S P1 C__S), beh__S (plug__S P2 C__S)))). *)
+  (* Proof. *)
+  (*   rewrite /τR2rhP. by rewrite [_ -> _] contra !neg_rhsat2. *)
+  (* Qed. *)
+
+  (* Lemma contra_τR2rHP : *)
+  (*   τR2rHP <-> (forall P1 P2 S, ((exists C__T,  ~ (τ S) (beh__T (plug__T (P1 ↓) C__T), *)
+  (*                                         beh__T (plug__T (P2 ↓) C__T ))) -> *)
+  (*                     (exists C__S, ~ S (beh__S (plug__S P1 C__S), beh__S (plug__S P2 C__S))))). *)
+  (* Proof. *)
+  (*   rewrite /τR2rHP. *)
+  (*   split => H P1 P2 S; by move/contra_τR2rhP: (H P1 P2 S). *)
+  (* Qed. *)
+
+  Lemma Galois_fst_lift (Hadj : Adjunction_law τ__π σ__π) :
+    forall T, SCH2 T ->
+       (sCl_τ (sCl_σ (T)) ⊆ T).
+  Admitted. 
+
+  Lemma Galois_snd_lift (Hadj : Adjunction_law τ__π σ__π) :
+    forall S, SCH2 S ->
+            S ⊆ (sCl_σ (sCl_τ S)).
+  Admitted. 
+  
+  Theorem Adj_sCl_σR2rSCHP_iff_sCl_τR2rSCHP :
+     Adjunction_law τ__π σ__π ->
+    (forall P1 P2 T, SCH2 T -> sCl_σR2rhP P1 P2 T) <->
+    (forall P1 P2 S, SCH2 S -> sCl_τR2rhP P1 P2 S).
+  Proof.
+    move => H_adj. split.
+    - move => Hσ P1 P2 S S_ssc Hrsat_src. 
+      have Hfoo: SCH2 (sCl_τ S) by apply: sCl2_SCH2.
+      have Hfoo': rsat__S P1 P2 (sCl_σ (sCl_τ S)). 
+      { apply: rhsat2_upper_closed.
+        exact Hrsat_src.
+        by apply: Galois_snd_lift. }         
+      by move: (Hσ P1 P2 (sCl_τ S) Hfoo Hfoo') => Hsat__T.  
+    - move => Hτ P1 P2 T T_ssc Hrrsat_tgt.
+      have H : rsat__T (P1 ↓) (P2 ↓) (sCl_τ (sCl_σ T)).
+      { apply: Hτ. apply: sCl2_SCH2. assumption. }
+      apply: rhsat2_upper_closed. exact H.
+      by apply: Galois_fst_lift.  
+  Qed.
+
+End Robust2relSSCHPreservation.
